checkpoint progress adding types to array

src/go_lang/array.v
@@ -2,7 +2,7 @@ From stdpp Require Import fin_maps.
 From iris.proofmode Require Import tactics.
 From iris.program_logic Require Export weakestpre.
 From Perennial.go_lang Require Export lifting.
-From Perennial.go_lang Require Import tactics notation.
+From Perennial.go_lang Require Import tactics notation typing.
 Set Default Proof Using "Type".
 
 (** This file defines the [array] connective, a version of [mapsto] that works
@@ -11,14 +11,15 @@ operations of HeapLand. *)
 
 Section go_lang.
   Context `{ffi_semantics: ext_semantics}.
+  Context {ext_tys:ext_types ext}.
   Context `{!ffi_interp ffi}.
 
 (* technically the definition of array doesn't depend on a state interp, only
 the ffiG type; fixing this would require unbundling ffi_interp *)
-Definition array `{!heapG Σ} (l : loc) (vs : list val) : iProp Σ :=
-  ([∗ list] i ↦ v ∈ vs, (l +ₗ i) ↦ Free v)%I.
-Notation "l ↦∗ vs" := (array l vs)
-  (at level 20, format "l  ↦∗  vs") : bi_scope.
+Definition array `{!heapG Σ} (l : loc) (t:ty) (vs : list val) : iProp Σ :=
+  ([∗ list] i ↦ v ∈ vs, (l +ₗ (i * ty_size t)) ↦[t] v)%I.
+Notation "l  ↦∗[ t ]  vs" := (array l t vs)
+  (at level 20) : bi_scope.
 
 (** We have no [FromSep] or [IntoSep] instances to remain forwards compatible
 with a fractional array assertion, that will split the fraction, not the
@@ -30,40 +31,44 @@ Implicit Types P Q : iProp Σ.
 Implicit Types Φ : val → iProp Σ.
 Implicit Types σ : state.
 Implicit Types v : val.
+Implicit Types t : ty.
 Implicit Types vs : list val.
 Implicit Types l : loc.
 Implicit Types sz off : nat.
 
-Global Instance array_timeless l vs : Timeless (array l vs) := _.
+Global Instance array_timeless l t vs : Timeless (array l t vs) := _.
 
-Lemma array_nil l : l ↦∗ [] ⊣⊢ emp.
+Lemma array_nil l t : l ↦∗[t] [] ⊣⊢ emp.
 Proof. by rewrite /array. Qed.
 
-Lemma array_singleton l v : l ↦∗ [v] ⊣⊢ l ↦ Free v.
+Lemma array_singleton l t v : l ↦∗[t] [v] ⊣⊢ l ↦[t] v.
 Proof. by rewrite /array /= right_id loc_add_0. Qed.
 
-Lemma array_app l vs ws :
-  l ↦∗ (vs ++ ws) ⊣⊢ l ↦∗ vs ∗ (l +ₗ length vs) ↦∗ ws.
+Lemma array_app l t vs ws :
+  l ↦∗[t] (vs ++ ws) ⊣⊢ l ↦∗[t] vs ∗ (l +ₗ length vs * ty_size t) ↦∗[t] ws.
 Proof.
   rewrite /array big_sepL_app.
   setoid_rewrite Nat2Z.inj_add.
-  by setoid_rewrite loc_add_assoc.
+  setoid_rewrite loc_add_assoc.
+  setoid_rewrite Z.mul_add_distr_r.
+  done.
 Qed.
 
-Lemma array_cons l v vs : l ↦∗ (v :: vs) ⊣⊢ l ↦ Free v ∗ (l +ₗ 1) ↦∗ vs.
+Lemma array_cons l v t vs : l ↦∗[t] (v :: vs) ⊣⊢ l ↦[t] v ∗ (l +ₗ ty_size t) ↦∗[t] vs.
 Proof.
   rewrite /array big_sepL_cons loc_add_0.
+  f_equiv.
   setoid_rewrite loc_add_assoc.
-  setoid_rewrite Nat2Z.inj_succ.
-  by setoid_rewrite Z.add_1_l.
+  assert (forall i, S i * ty_size t = ty_size t + i * ty_size t) as Hoff; [ lia | ].
+  by setoid_rewrite Hoff.
 Qed.
 
-Lemma update_array l vs off v :
+Lemma update_array l vs off t v :
   vs !! off = Some v →
-  (l ↦∗ vs -∗ ((l +ₗ off) ↦ Free v ∗ ∀ v', (l +ₗ off) ↦ Free v' -∗ l ↦∗ <[off:=v']>vs))%I.
+  (l ↦∗[t] vs -∗ ((l +ₗ off * ty_size t) ↦[t] v ∗ ∀ v', (l +ₗ off * ty_size t) ↦[t] v' -∗ l ↦∗[t] <[off:=v']>vs))%I.
 Proof.
   iIntros (Hlookup) "Hl".
-  rewrite -[X in (l ↦∗ X)%I](take_drop_middle _ off v); last done.
+  rewrite -[X in (l ↦∗[_] X)%I](take_drop_middle _ off v); last done.
   iDestruct (array_app with "Hl") as "[Hl1 Hl]".
   iDestruct (array_cons with "Hl") as "[Hl2 Hl3]".
   assert (off < length vs)%nat as H by (apply lookup_lt_is_Some; by eexists).
@@ -71,44 +76,51 @@ Proof.
   iIntros (w) "Hl2".
   clear Hlookup. assert (<[off:=w]> vs !! off = Some w) as Hlookup.
   { apply list_lookup_insert. lia. }
-  rewrite -[in (l ↦∗ <[off:=w]> vs)%I](take_drop_middle (<[off:=w]> vs) off w Hlookup).
+  rewrite -[in (l ↦∗[_] <[off:=w]> vs)%I](take_drop_middle (<[off:=w]> vs) off w Hlookup).
   iApply array_app. rewrite take_insert; last by lia. iFrame.
   iApply array_cons. rewrite take_length min_l; last by lia. iFrame.
   rewrite drop_insert; last by lia. done.
 Qed.
 
 (** Allocation *)
-Lemma mapsto_seq_array l v n :
-  ([∗ list] i ∈ seq 0 n, (l +ₗ (i : nat)) ↦ Free v) -∗
-  l ↦∗ replicate n v.
+Lemma mapsto_seq_array l v t n :
+  ([∗ list] i ∈ seq 0 n, (l +ₗ (i : nat) * ty_size t) ↦[t] v) -∗
+  l ↦∗[t] replicate n v.
 Proof.
   rewrite /array. iInduction n as [|n'] "IH" forall (l); simpl.
   { done. }
   iIntros "[$ Hl]". rewrite -fmap_seq big_sepL_fmap.
   setoid_rewrite Nat2Z.inj_succ. setoid_rewrite <-Z.add_1_l.
+  setoid_rewrite Z.mul_add_distr_r.
+  setoid_rewrite Z.mul_1_l.
   setoid_rewrite <-loc_add_assoc. iApply "IH". done.
 Qed.
 
-Lemma mapsto_seq_struct_array l v n :
-  ([∗ list] i ∈ seq 0 n, (l +ₗ (i * length (flatten_struct v))%nat) ↦s v) -∗
-  l ↦∗ concat_replicate n (flatten_struct v).
+Lemma Zmul_S_l (n: nat) z : S n * z = z + n * z.
+Proof.
+  lia.
+Qed.
+
+Lemma mapsto_seq_struct_array l v t n :
+  ([∗ list] i ∈ seq 0 n, (l +ₗ ((i:nat) * ty_size t)) ↦[t] v) -∗
+  l ↦∗[t] replicate n v.
 Proof.
   rewrite /array. iInduction n as [|n'] "IH" forall (l); simpl.
   { done. }
-  rewrite concat_replicate_S loc_add_0.
+  rewrite loc_add_0.
   iIntros "[$ Hl]". rewrite -fmap_seq big_sepL_fmap.
-  simpl.
-  setoid_rewrite Nat2Z.inj_add.
+  setoid_rewrite Zmul_S_l.
   setoid_rewrite <-loc_add_assoc.
   iApply "IH". done.
 Qed.
 
-Lemma wp_allocN s E v (n: u64) :
+Lemma wp_allocN s E v t (n: u64) :
   (0 < int.val n)%Z →
+  val_ty v t ->
   {{{ True }}} AllocN (Val $ LitV $ LitInt $ n) (Val v) @ s; E
-  {{{ l, RET LitV (LitLoc l); l ↦∗ concat_replicate (int.nat n) (flatten_struct v) }}}.
+  {{{ l, RET LitV (LitLoc l); l ↦∗[t] replicate (int.nat n) v }}}.
 Proof.
-  iIntros (Hzs Φ) "_ HΦ". iApply wp_allocN_seq; [done..|]. iNext.
+  iIntros (Hsz Hty Φ) "_ HΦ". iApply wp_allocN_seq; [done..|]. iNext.
   iIntros (l) "Hlm". iApply "HΦ".
   by iApply mapsto_seq_struct_array.
 Qed.
@@ -151,21 +163,27 @@ Qed.
 
 (** Access to array elements *)
 
-Lemma wp_load_offset s E l off vs v :
+(* not true - only holds for type-based load at t *)
+Lemma wp_load_offset s E l off t vs v :
   vs !! off = Some v →
-  {{{ ▷ l ↦∗ vs }}} ! #(l +ₗ off) @ s; E {{{ RET v; l ↦∗ vs }}}.
+  {{{ ▷ l ↦∗[t] vs }}} ! #(l +ₗ off * ty_size t) @ s; E {{{ RET v; l ↦∗[t] vs }}}.
 Proof.
   iIntros (Hlookup Φ) "Hl HΦ".
-  iDestruct (update_array l _ _ _ Hlookup with "Hl") as "[Hl1 Hl2]".
+  iDestruct (update_array l _ _ _ _ Hlookup with "Hl") as "[Hl1 Hl2]".
+  (*
   iApply (wp_load with "Hl1"). iIntros "!> Hl1". iApply "HΦ".
   iDestruct ("Hl2" $! v) as "Hl2". rewrite list_insert_id; last done.
   iApply "Hl2". iApply "Hl1".
-Qed.
+   *)
+Abort.
 
+(*
 Lemma wp_load_offset_vec s E l sz (off : fin sz) (vs : vec val sz) :
   {{{ ▷ l ↦∗ vs }}} ! #(l +ₗ off) @ s; E {{{ RET vs !!! off; l ↦∗ vs }}}.
 Proof. apply wp_load_offset. by apply vlookup_lookup. Qed.
+*)
 
+(*
 Lemma wp_cmpxchg_suc_offset s E l off vs v' v1 v2 :
   vs !! off = Some v' →
   v' = v1 →
@@ -214,10 +232,11 @@ Lemma wp_cmpxchg_fail_offset_vec s E l sz (off : fin sz) (vs : vec val sz) v1 v2
     CmpXchg #(l +ₗ off) v1 v2 @ s; E
   {{{ RET (vs !!! off, #false); l ↦∗ vs }}}.
 Proof. intros. eapply wp_cmpxchg_fail_offset=> //. by apply vlookup_lookup. Qed.
+*)
 
 End lifting.
 End go_lang.
 
-Notation "l ↦∗ vs" := (array l vs)
-  (at level 20, format "l  ↦∗  vs") : bi_scope.
+Notation "l  ↦∗[ t ]  vs" := (array l t vs)
+  (at level 20) : bi_scope.
 Typeclasses Opaque array.
